qa/lean/Ragu/Instances/Element/DivNonzero.lean
@@ -7,7 +7,7 @@ open Ragu.Instances.Autogen.Element.DivNonzero
 
 def deserializeInput (input : Vector (Expression (F p)) inputLen) :
     Var Circuits.Element.DivNonzero.Input (F p) :=
-  { x := input[0], y := input[1] }
+  { x := input[0], y := input[1], inverse := fun _ => 0 }
 
 def serializeOutput (output : Var field (F p)) : Vector (Expression (F p)) 1 :=
   #v[output]
@@ -20,30 +20,21 @@ def formal_instance : Core.Statements.FormalInstance where
   deserializeInput
   serializeOutput
 
-  reimplementation := Circuits.Element.DivNonzero.circuit.toWithHint
+  reimplementation := Circuits.Element.DivNonzero.circuit
 
   same_constraints := by
     intro input
     simp [Core.Statements.FlatOperation.eraseCompute, List.map,
       Operations.toFlat, circuit_norm,
-      GeneralFormalCircuit.toWithHint,
       GeneralFormalCircuit.WithHint.toSubcircuit,
       deserializeInput, exportedOperations,
       Circuits.Element.DivNonzero.circuit,
       Circuits.Element.DivNonzero.elaborated,
       Circuits.Element.DivNonzero.main,
       Circuits.Core.Mul.main]
-    repeat (constructor; rfl)
-    constructor
+    refine ⟨?_, ?_, ?_, ?_, ?_, ?_⟩ <;> rfl
   same_output := by
     intro input
-    simp [circuit_norm,
-      GeneralFormalCircuit.toWithHint,
-      GeneralFormalCircuit.WithHint.toSubcircuit,
-      deserializeInput, serializeOutput,
-      Circuits.Element.DivNonzero.circuit,
-      Circuits.Element.DivNonzero.elaborated,
-      Circuits.Element.DivNonzero.main,
-      Circuits.Core.Mul.main]
+    rfl
 
 end Ragu.Instances.Element.DivNonzero
