qa/lean/Ragu/Instances/Element/EnforceNonzero.lean
@@ -1,16 +1,16 @@
-import Ragu.Circuits.Element.InvertWith
-import Ragu.Instances.Autogen.Element.InvertWith
+import Ragu.Circuits.Element.EnforceNonzero
+import Ragu.Instances.Autogen.Element.EnforceNonzero
 import Ragu.Core
 
-namespace Ragu.Instances.Element.InvertWith
-open Ragu.Instances.Autogen.Element.InvertWith
+namespace Ragu.Instances.Element.EnforceNonzero
+open Ragu.Instances.Autogen.Element.EnforceNonzero
 
 def deserializeInput (input : Vector (Expression (F p)) inputLen) :
-    Var Circuits.Element.InvertWith.Input (F p) :=
+    Var Circuits.Element.EnforceNonzero.Input (F p) :=
   { input := input[0], inverse := fun _ => 0 }
 
-def serializeOutput (output : Var field (F p)) : Vector (Expression (F p)) 1 :=
-  #v[output]
+def serializeOutput (_output : Var unit (F p)) : Vector (Expression (F p)) 0 :=
+  #v[]
 
 def formal_instance : Core.Statements.FormalInstance where
   p
@@ -20,7 +20,7 @@ def formal_instance : Core.Statements.FormalInstance where
   deserializeInput
   serializeOutput
 
-  reimplementation := Circuits.Element.InvertWith.circuit
+  reimplementation := Circuits.Element.EnforceNonzero.circuit
 
   same_constraints := by
     intro input
@@ -28,13 +28,13 @@ def formal_instance : Core.Statements.FormalInstance where
       Operations.toFlat, circuit_norm,
       GeneralFormalCircuit.WithHint.toSubcircuit,
       deserializeInput, exportedOperations,
-      Circuits.Element.InvertWith.circuit,
-      Circuits.Element.InvertWith.elaborated,
-      Circuits.Element.InvertWith.main,
+      Circuits.Element.EnforceNonzero.circuit,
+      Circuits.Element.EnforceNonzero.elaborated,
+      Circuits.Element.EnforceNonzero.main,
       Circuits.Core.Mul.main]
     refine ⟨?_, ?_, ?_⟩ <;> rfl
   same_output := by
     intro input
     rfl
 
-end Ragu.Instances.Element.InvertWith
+end Ragu.Instances.Element.EnforceNonzero
