qa/lean/Ragu/Instances/NonzeroBank/ScopeK2.lean
@@ -1,0 +1,46 @@
+import Ragu.Circuits.NonzeroBank.ScopeK2
+import Ragu.Instances.Autogen.NonzeroBank.ScopeK2
+import Ragu.Core
+
+namespace Ragu.Instances.NonzeroBank.ScopeK2
+open Ragu.Instances.Autogen.NonzeroBank.ScopeK2
+
+def deserializeInput (input : Vector (Expression (F p)) inputLen) :
+    Var Circuits.NonzeroBank.ScopeK2.Input (F p) :=
+  { f1 := input[0], f2 := input[1], inverse := fun _ => 0 }
+
+def serializeOutput (_output : Var unit (F p)) : Vector (Expression (F p)) 0 :=
+  #v[]
+
+def formal_instance : Core.Statements.FormalInstance where
+  p
+  exportedOperations
+  exportedOutput
+
+  deserializeInput
+  serializeOutput
+
+  reimplementation := Circuits.NonzeroBank.ScopeK2.circuit
+
+  same_constraints := by
+    intro input
+    simp [Core.Statements.FlatOperation.eraseCompute, List.map,
+      Operations.toFlat, circuit_norm,
+      GeneralFormalCircuit.WithHint.toSubcircuit, FormalCircuit.toSubcircuit,
+      deserializeInput, exportedOperations,
+      Circuits.NonzeroBank.ScopeK2.circuit,
+      Circuits.NonzeroBank.ScopeK2.elaborated,
+      Circuits.NonzeroBank.ScopeK2.main,
+      Circuits.Element.Mul.circuit,
+      Circuits.Element.Mul.elaborated,
+      Circuits.Element.Mul.main,
+      Circuits.Element.EnforceNonzero.circuit,
+      Circuits.Element.EnforceNonzero.elaborated,
+      Circuits.Element.EnforceNonzero.main,
+      Circuits.Core.Mul.main]
+    refine ⟨?_, ?_, ?_, ?_, ?_, ?_, ?_, ?_, ?_⟩ <;> rfl
+  same_output := by
+    intro input
+    rfl
+
+end Ragu.Instances.NonzeroBank.ScopeK2
