qa/lean/Ragu/Instances/Point/DoubleAndAddIncomplete.lean
@@ -8,7 +8,8 @@ open Ragu.Instances.Autogen.Point.DoubleAndAddIncomplete
 def deserializeInput (input : Vector (Expression (F p)) inputLen)
     : Var Circuits.Point.DoubleAndAddIncomplete.Inputs (F p) :=
   { P1 := { x := input[0], y := input[1] },
-    P2 := { x := input[2], y := input[3] } }
+    P2 := { x := input[2], y := input[3] },
+    inverse := fun _ => 0 }
 
 def serializeOutput (output : Var Circuits.Point.Spec.Point (F p))
     : Vector (Expression (F p)) 2 :=
@@ -24,52 +25,35 @@ def formal_instance : Core.Statements.FormalInstance where
   serializeOutput
 
   reimplementation :=
-    (Circuits.Point.DoubleAndAddIncomplete.circuit Circuits.Point.Spec.EpAffineParams).toWithHint
+    Circuits.Point.DoubleAndAddIncomplete.circuit Circuits.Point.Spec.EpAffineParams
 
   same_constraints := by
     intro input
     simp [Core.Statements.FlatOperation.eraseCompute, List.map,
-      Operations.toFlat, circuit_norm, exportedOperations,
-      GeneralFormalCircuit.toSubcircuit, GeneralFormalCircuit.toWithHint,
-      GeneralFormalCircuit.WithHint.toSubcircuit,
-      FormalCircuit.toSubcircuit,
-      deserializeInput,
+      Operations.toFlat, circuit_norm,
+      GeneralFormalCircuit.WithHint.toSubcircuit, FormalCircuit.toSubcircuit,
+      GeneralFormalCircuit.toSubcircuit,
+      deserializeInput, exportedOperations,
       Circuits.Point.DoubleAndAddIncomplete.circuit,
       Circuits.Point.DoubleAndAddIncomplete.elaborated,
       Circuits.Point.DoubleAndAddIncomplete.main,
-      Circuits.Element.DivNonzero.circuit,
-      Circuits.Element.DivNonzero.elaborated,
-        Circuits.Element.DivNonzero.main,
-      Circuits.Element.Square.circuit,
-      Circuits.Element.Square.elaborated,
-      Circuits.Element.Square.main,
       Circuits.Element.Mul.circuit,
       Circuits.Element.Mul.elaborated,
       Circuits.Element.Mul.main,
+      Circuits.Element.Divide.circuit,
+      Circuits.Element.Divide.elaborated,
+      Circuits.Element.Divide.main,
+      Circuits.Element.Square.circuit,
+      Circuits.Element.Square.elaborated,
+      Circuits.Element.Square.main,
+      Circuits.Element.EnforceNonzero.circuit,
+      Circuits.Element.EnforceNonzero.elaborated,
+      Circuits.Element.EnforceNonzero.main,
       Circuits.Core.Mul.main]
-    repeat (constructor; rfl)
-    constructor
+    refine ⟨?_, ?_, ?_, ?_, ?_, ?_, ?_, ?_, ?_, ?_, ?_, ?_,
+            ?_, ?_, ?_, ?_, ?_, ?_, ?_, ?_, ?_, ?_, ?_, ?_⟩ <;> rfl
   same_output := by
     intro input
-    simp [circuit_norm,
-      GeneralFormalCircuit.toSubcircuit, GeneralFormalCircuit.toWithHint,
-      GeneralFormalCircuit.WithHint.toSubcircuit,
-      FormalCircuit.toSubcircuit,
-      deserializeInput, serializeOutput,
-      Circuits.Point.DoubleAndAddIncomplete.circuit,
-      Circuits.Point.DoubleAndAddIncomplete.elaborated,
-      Circuits.Point.DoubleAndAddIncomplete.main,
-      Circuits.Element.DivNonzero.circuit,
-      Circuits.Element.DivNonzero.elaborated,
-        Circuits.Element.DivNonzero.main,
-      Circuits.Element.Square.circuit,
-      Circuits.Element.Square.elaborated,
-      Circuits.Element.Square.main,
-      Circuits.Element.Mul.circuit,
-      Circuits.Element.Mul.elaborated,
-      Circuits.Element.Mul.main,
-      Circuits.Core.Mul.main]
-    refine ⟨?_, rfl⟩
     rfl
 
 end Ragu.Instances.Point.DoubleAndAddIncomplete
